Makefile
@@ -1,12 +1,32 @@
 civl = boogie -noinfer -typeEncoding:m -useArrayTheory
-impls = $(wildcard lib/impls/*.bpl)
-targets = $(patsubst lib/impls/%.bpl,%,$(impls))
+adts = $(patsubst lib/adts/%.bpl,%,$(wildcard lib/adts/*.bpl))
+impls = $(patsubst lib/impls/%.bpl,%,$(wildcard lib/impls/*.bpl))
 prelude = $(wildcard lib/prelude/*.bpl)
 
-all: $(targets)
+.PHONY: all checks prelude-checks adt-checks $(adts)
+
+all: checks $(impls)
+
+checks: prelude-checks adt-checks
+
+prelude-checks:
+	@echo Checking prelude
+	@echo ---
+	@boogie lib/prelude/invocations.bpl
+	@echo ---
+	@boogie lib/prelude/*.bpl
+	@echo ---
+
+adt-checks: $(adts)
+
+$(adts): %: lib/adts/%.bpl
+	@echo Checking ADT: $@
+	@echo ---
+	boogie lib/prelude/*.bpl $<
+	@echo ---
 
 .SECONDEXPANSION:
-$(targets): %: $(prelude) lib/adts/$$(lastword $$(subst -, ,$$@)).bpl lib/impls/%.bpl
+$(impls): %: $(prelude) lib/adts/$$(lastword $$(subst -, ,$$@)).bpl lib/impls/%.bpl
 	@echo Verifying implementation: $@
 	@echo ---
 	$(civl) $^
